Added tactics for substitutions. These work on the modular funcs.

MirrorCharge!/src/MirrorCharge/Java/JavaFunc.v
@@ -40,12 +40,11 @@ Set Strict Implicit.
 
 
 	Inductive java_func :=
-	| pVar (_ : var)
 	| pField (_ : field)
 	| pClass (_ : class)
-	| pVal (_ : sval)
+	| pVal (_ : val)
 	| pVarList (_ : list var) 
-	| pProg (_ : Prog_wf)
+	| pProg (_ : Program)
 	| pCmd (_ : cmd)
 	| pDExpr (_ : dexpr)
 	| pFields (_ : SS.t)
@@ -54,14 +53,22 @@ Set Strict Implicit.
 	| pProgEq
 	| pTriple
 	| pTypeOf
-	| pEval
 	| pFieldLookup
 	
 	| pSetFold (_ : typ)
 	| pSetFoldFun 
 	
 	| pPointsto
-	| pNull.
+	| pNull
+	
+	| pPlus
+	| pMinus
+	| pTimes
+	| pAnd
+	| pOr
+	| pNot
+	| pLt
+	| pValEq.
 
 	Fixpoint beq_list {A} (f : A -> A -> bool) (xs ys : list A) :=
 		match xs, ys with
@@ -72,7 +79,6 @@ Set Strict Implicit.
 
 	Definition typeof_java_func bf :=
 		match bf with
-		    | pVar _ => Some tyVar
 		    | pField _ => Some tyField
 		    | pClass _ => Some tyClass
 		    | pVal _ => Some tyVal
@@ -86,7 +92,6 @@ Set Strict Implicit.
 		    	 (tyArr tyVar (tyArr tySasn (tyArr tySasn tySpec))))))
 		    | pProgEq => Some (tyArr tyProg tySpec)
 		    | pTriple => Some (tyArr tySasn (tyArr tySasn (tyArr tyCmd tySpec)))
-		    | pEval => Some (tyArr tyDExpr tyExpr)
 		    
 		    | pTypeOf => Some (tyArr tyVar (tyArr tyVal tyProp))
 		    
@@ -98,11 +103,19 @@ Set Strict Implicit.
 		    | pPointsto => Some (tyArr tyVal (tyArr tyField (tyArr tyVal tyAsn)))
 		    
 		    | pNull => Some tyVal
+		    
+		    | pPlus => Some (tyArr tyVal (tyArr tyVal tyVal))
+		    | pMinus => Some (tyArr tyVal (tyArr tyVal tyVal))
+		    | pTimes => Some (tyArr tyVal (tyArr tyVal tyVal))
+		    | pAnd => Some (tyArr tyVal (tyArr tyVal tyVal))
+		    | pOr => Some (tyArr tyVal (tyArr tyVal tyVal))
+		    | pNot => Some (tyArr tyVal tyVal)
+		    | pLt => Some (tyArr tyVal (tyArr tyVal tyVal))
+		    | pValEq => Some (tyArr tyVal (tyArr tyVal tyVal))
 		end.
 
 	Definition java_func_eq (a b : java_func) : option bool :=
 	  match a , b with
-	    | pVar a, pVar b => Some (a ?[ eq ] b)
 	    | pField a, pField b => Some (a ?[ eq ] b)
 	    | pClass a, pClass b => Some (a ?[ eq ] b)
 		| pVal a, pVal b => Some (beq_val a b)
@@ -118,14 +131,20 @@ Set Strict Implicit.
 	
 	    | pTypeOf, pTypeOf => Some true
 	
-		| pEval, pEval => Some true
-	
 	    | pPointsto, pPointsto => Some true
 	    | pFieldLookup, pFieldLookup => Some true
 	    | pSetFold t, pSetFold u => Some (t ?[ eq ] u)
 	    | pSetFoldFun, pSetFoldFun => Some true
 	
 	    | pNull, pNull => Some true
+	    | pPlus, pPlus => Some true
+	    | pMinus, pMinus => Some true
+	    | pTimes, pTimes => Some true
+	    | pAnd, pAnd => Some true
+	    | pOr, pOr => Some true
+	    | pNot, pNot => Some true
+	    | pLt, pLt => Some true
+	    | pValEq, pValEq => Some true
 	    | _, _ => None
 	  end.
 
@@ -153,7 +172,6 @@ Definition set_fold_fun (x : String.string) (f : field) (P : sasn) :=
 								| Some t => typD t
 								| None => unit
 							  end with
-              | pVar v => v
               | pClass c => c
               | pField f => f
               | pProg p => p
@@ -166,7 +184,6 @@ Definition set_fold_fun (x : String.string) (f : field) (P : sasn) :=
               | pMethodSpec => method_spec
               | pProgEq => prog_eq
               | pTriple => triple
-              | pEval => eval
               
               | pTypeOf => typeof
                             
@@ -177,6 +194,15 @@ Definition set_fold_fun (x : String.string) (f : field) (P : sasn) :=
               | pPointsto => pointsto
               
               | pNull => null
+              
+              | pPlus => eplus
+              | pMinus => eminus
+              | pTimes => etimes
+              | pAnd => eand
+              | pOr => eor
+              | pNot => enot
+              | pLt => elt
+              | pValEq => eeq
 	end.
 
 	Global Instance RSym_JavaFunc : SymI.RSym java_func := {
@@ -201,11 +227,10 @@ Definition set_fold_fun (x : String.string) (f : field) (P : sasn) :=
 	Qed.
 
 Definition func := (SymEnv.func + @ilfunc typ + @bilfunc typ + 
-                    @base_func typ + @list_func typ + @open_func typ + 
+                    @base_func typ + @list_func typ + @open_func typ _ _ + 
                     @embed_func typ + @later_func typ + java_func)%type.
 
 Section MakeJavaFunc.
-	Definition mkVar v : expr typ func := Inj (inr (pVar v)).
 	Definition mkField f : expr typ func := Inj (inr (pField f)).
 	Definition mkClass c : expr typ func := Inj (inr (pClass c)).
 	Definition mkVal v : expr typ func := Inj (inr (pVal v)).
@@ -219,12 +244,20 @@ Section MakeJavaFunc.
 	Definition fProgEq : expr typ func := Inj (inr pProgEq).
 	Definition fTriple : expr typ func := Inj (inr pTriple).
 	Definition fTypeOf : expr typ func := Inj (inr pTypeOf).
-	Definition fEval : expr typ func := Inj (inr pEval).
 	Definition fFieldLookup : expr typ func := Inj (inr pFieldLookup).
 	Definition fSetFold t : expr typ func := Inj (inr (pSetFold t)).
 	Definition fSetFoldFun : expr typ func := Inj (inr pSetFoldFun).
 	Definition fPointsto : expr typ func := Inj (inr pPointsto).
 	Definition mkNull : expr typ func := Inj (inr pNull).
+
+	Definition fPlus : expr typ func := Inj (inr pPlus).
+	Definition fMinus : expr typ func := Inj (inr pMinus).
+	Definition fTimes : expr typ func := Inj (inr pTimes).
+	Definition fAnd : expr typ func := Inj (inr pAnd).
+	Definition fOr : expr typ func := Inj (inr pOr).
+	Definition fNot : expr typ func := Inj (inr pNot).
+	Definition fLt : expr typ func := Inj (inr pLt).
+	Definition fValEq : expr typ func := Inj (inr pValEq).
 
 	Definition mkTriple P c Q : expr typ func := App (App (App fTriple P) Q) c.
 	Definition mkFieldLookup P C f : expr typ func := App (App (App fFieldLookup P) C) f.
@@ -236,15 +269,22 @@ Section MakeJavaFunc.
 		(fold_right (fun (e : dexpr) (acc : expr typ func) => 
 			mkCons tyExpr (mkDExpr e) acc) (mkNil tyExpr) es).
 	
-	Definition mkEval e s := App (App fEval e) s.
+
+	Fixpoint evalDExpr (e : dexpr) : expr typ func :=
+		match e with
+			| E_val v => mkConst tyVal (mkVal v)
+			| E_var x => App (fStackGet (func := expr typ func)) (mkVar (func := func) x)
+			| E_plus e1 e2 => mkAps fPlus ((evalDExpr e2, tyVal)::(evalDExpr e1, tyVal)::nil) tyVal
+			| E_minus e1 e2 => mkAps fMinus ((evalDExpr e2, tyVal)::(evalDExpr e1, tyVal)::nil) tyVal
+			| E_times e1 e2 => mkAps fTimes ((evalDExpr e2, tyVal)::(evalDExpr e1, tyVal)::nil) tyVal
+			| E_and e1 e2 => mkAps fAnd ((evalDExpr e2, tyVal)::(evalDExpr e1, tyVal)::nil) tyVal
+			| E_or e1 e2 => mkAps fOr ((evalDExpr e2, tyVal)::(evalDExpr e1, tyVal)::nil) tyVal
+			| E_not e => mkAps fNot ((evalDExpr e, tyVal)::nil) tyVal
+			| E_lt e1 e2 => mkAps fLt ((evalDExpr e2, tyVal)::(evalDExpr e1, tyVal)::nil) tyVal
+			| E_eq e1 e2 => mkAps fValEq ((evalDExpr e2, tyVal)::(evalDExpr e1, tyVal)::nil) tyVal
+		end.
 
 End MakeJavaFunc.
-
-Example test : expr typ func := mkStar tySasn (mkFalse tySasn) (mkTrue tySasn).
-
-Eval vm_compute in test.
-
-Print RSym.
 
 Definition fs : @SymEnv.functions typ _ := SymEnv.from_list nil.
 Locate RSym_func.
@@ -259,8 +299,8 @@ Instance RSym_embed_func : RSym (@embed_func typ) :=
 Instance RSym_later_func : RSym (@later_func typ) :=
 	RSym_later_func _ lops.
 	Check null.
-Instance RSym_open_func : RSym (@open_func typ) :=
-	@RSym_OpenFunc _ _ _ RType_typ _ _ tyVar tyVal _ null _ _ _ _.
+Instance RSym_open_func : RSym (@open_func typ _ _) :=
+	@RSym_OpenFunc _ _ _ RType_typ _ _ _ _ _ _ _ _.
 
 Existing Instance RSym_sum.
 Existing Instance RSymOk_sum.
@@ -278,6 +318,22 @@ Instance SU : SubstI.SubstUpdate subst (expr typ func) :=
   FMapSubst.SUBST.SubstUpdate_subst (@instantiate typ func).
 Instance SO : SubstI.SubstOk Expr_expr SS := 
   @FMapSubst.SUBST.SubstOk_subst typ RType_typ (expr typ func) _ _.
+
+Lemma evalDexpr_wt (e : dexpr) : 
+	typeof_expr nil nil (evalDExpr e) = Some tyExpr. 
+Proof.
+  induction e.
+  + simpl; reflexivity.
+  + simpl; reflexivity.
+  + simpl; rewrite IHe1, IHe2; reflexivity.
+  + simpl; rewrite IHe1, IHe2; reflexivity.
+  + simpl; rewrite IHe1, IHe2; reflexivity.
+  + simpl; rewrite IHe1, IHe2; reflexivity.
+  + simpl; rewrite IHe1, IHe2; reflexivity.
+  + simpl; rewrite IHe; reflexivity.
+  + simpl; rewrite IHe1, IHe2; reflexivity.
+  + simpl; rewrite IHe1, IHe2; reflexivity.
+Qed.
 
 Definition test_lemma :=
   @lemmaD typ RType_typ (expr typ func) Expr_expr (expr typ func)
