MirrorCharge!/src/MirrorCharge/ModularFunc/OpenFunc.v
@@ -24,9 +24,26 @@ Set Implicit Arguments.
 Set Strict Implicit.
 Set Maximal Implicit Insertion.
 
-Class OpenFunc (typ func : Type) := {
+  Inductive open_func typ {RType_typ : RType typ} {HST : SubstType typ} :=
+    | of_const (_ : typ)
+    | of_ap (_ _ : typ)
+    | of_var (_ : typD tyVar)
+    | of_null
+    | of_stack_get
+    | of_stack_set
+    | of_apply_subst (_ : typ)
+    | of_single_subst
+    | of_subst
+    | of_trunc_subst.
+    
+Implicit Arguments open_func [[RType_typ] [HST]].
+    
+Class OpenFunc (typ func : Type) {RType_typ : RType typ} {HST : SubstType typ} := {
   fConst : typ -> func;
   fAp : typ -> typ -> func;
+  
+  fVar : typD tyVar -> func;
+  fNull : func;
   
   fStackGet : func;
   fStackSet : func;
@@ -34,16 +51,23 @@ Class OpenFunc (typ func : Type) := {
   fApplySubst : typ -> func;
   fSingleSubst : func;
   fSubst : func;
-  fTruncSubst : func
+  fTruncSubst : func;
+  
+  open_funcS : func -> option (open_func typ)
 }.
-    
+
+Implicit Arguments OpenFunc [[RType_typ] [HST]].
+
 Section OpenFuncSum.
-	Context {typ func : Type} {H : OpenFunc typ func}.
+	Context {typ func : Type} `{H : OpenFunc typ func}.
 
 	Global Instance OpenFuncSumL (A : Type) : 
 	   OpenFunc typ (func + A) := {
 		  fConst t := inl (fConst t);
 		  fAp t u := inl (fAp t u);
+		  
+		  fVar x := inl (fVar x);
+		  fNull := inl fNull;
 		  
 		  fStackGet := inl fStackGet;
 		  fStackSet := inl fStackSet;
@@ -51,7 +75,12 @@ Section OpenFuncSum.
 		  fApplySubst t := inl (fApplySubst t);
 		  fSingleSubst := inl fSingleSubst;
 		  fSubst := inl fSubst;
-		  fTruncSubst := inl fTruncSubst
+		  fTruncSubst := inl fTruncSubst;
+		  
+		  open_funcS f := match f with
+		  				    | inl f => open_funcS f
+		  				    | inr _ => None
+		  				  end
        }.
 
 	Global Instance OpenFuncSumR (A : Type) : 
@@ -59,13 +88,22 @@ Section OpenFuncSum.
 		  fConst t := inr (fConst t);
 		  fAp t u := inr (fAp t u);
 		  
+		  fVar x := inr (fVar x);
+		  fNull := inr fNull;
+		  
 		  fStackGet := inr fStackGet;
 		  fStackSet := inr fStackSet;
 		  
 		  fApplySubst t := inr (fApplySubst t);
 		  fSingleSubst := inr fSingleSubst;
 		  fSubst := inr fSubst;
-		  fTruncSubst := inr fTruncSubst
+		  fTruncSubst := inr fTruncSubst;
+		  
+		  open_funcS f := match f with
+		  				    | inr f => open_funcS f
+		  				    | inl _ => None
+		  				  end
+		  
        }.
 
 	Global Instance OpenFuncExpr : 
@@ -73,13 +111,22 @@ Section OpenFuncSum.
 		  fConst t := Inj (fConst t);
 		  fAp t u := Inj (fAp t u);
 		  
+		  fVar x := Inj (fVar x);
+		  fNull := Inj fNull;
+		  
 		  fStackGet := Inj fStackGet;
 		  fStackSet := Inj fStackSet;
 		  
 		  fApplySubst t := Inj (fApplySubst t);
 		  fSingleSubst := Inj fSingleSubst;
 		  fSubst := Inj fSubst;
-		  fTruncSubst := Inj fTruncSubst
+		  fTruncSubst := Inj fTruncSubst;
+		  
+		  open_funcS f := match f with
+		  				    | Inj f => open_funcS f
+		  				    | _ => None
+		  				  end
+		  
        }.
 
 End OpenFuncSum.
@@ -92,60 +139,59 @@ Section OpenFuncInst.
     Variable Typ2_tyArr : Typ2 _ Fun.
     Variable Typ0_tyProp : Typ0 _ Prop.
     
-    Context {d r : typ} {Hd : DecidableEq (typD d)} (null : typD r).
-    Context {Hst : SubstType typ} {HstD: @SubstTypeD typ _ _ d r null}.
+    Context {HST : SubstType typ} {HV : ValNull (typD tyVal)}.
+    Context {HSTD : SubstTypeD}.
     Context {HBTD : BaseTypeD} {HLTD : ListTypeD}.
     
+	Context {RelDec_var : RelDec (@eq (typD tyVar))}.
+	Context {RelDec_var_Correct : RelDec_Correct RelDec_var}.
+	
     Let tyArr : typ -> typ -> typ := @typ2 _ _ _ _.
     Let tyProp : typ := @typ0 _ _ _ _.
 
-	Local Notation "'tyStack'" := (tyArr d r).
-	Local Notation "'tyExpr'" := (tyArr tyStack r).
-	Local Notation "'tySubstList'" := (tyList (tyPair d (tyArr tyStack r))).
+	Local Notation "'tyStack'" := (tyArr tyVar tyVal).
+	Local Notation "'tyExpr'" := (tyArr tyStack tyVal).
+	Local Notation "'tySubstList'" := (tyList (tyPair tyVar (tyArr tyStack tyVal))).
 
-	Definition stack := @stack (typD d) (@VN typ _ r null).
+	Definition stack := @stack (typD tyVar) (typD tyVal).
 
-  Inductive open_func :=
-    | of_const (_ : typ)
-    | of_ap (_ _ : typ)
-    | of_stack_get
-    | of_stack_set
-    | of_apply_subst (_ : typ)
-    | of_single_subst
-    | of_subst
-    | of_trunc_subst.
-    
-	Global Instance LaterFuncInst : OpenFunc typ open_func := {
+	Global Instance LaterFuncInst : OpenFunc typ (open_func typ) := {
 	  fConst := of_const;
 	  fAp := of_ap;
+	  fVar := of_var;
+	  fNull := of_null;
 	  fStackGet := of_stack_get;
 	  fStackSet := of_stack_set;
 	  fApplySubst := of_apply_subst;
 	  fSingleSubst := of_single_subst;
 	  fSubst := of_subst;
-	  fTruncSubst := of_trunc_subst
+	  fTruncSubst := of_trunc_subst;
+	  
+	  open_funcS f := Some f
 	}.
-	
   
-  Definition typeof_open_func (f : open_func) : option typ :=
+  Definition typeof_open_func (f : open_func typ) : option typ :=
     match f with
     | of_const t => Some (tyArr t (tyArr tyStack t))
     | of_ap t u => Some (tyArr (tyArr tyStack (tyArr t u)) (tyArr (tyArr tyStack t) (tyArr tyStack u)))
     | of_apply_subst t => Some (tyArr (tyArr tyStack t) (tyArr tySubst (tyArr tyStack t)))
-
-    | of_stack_get => Some (tyArr d tyExpr)
-    | of_stack_set => Some (tyArr d (tyArr r (tyArr tyStack tyStack)))
-    | of_single_subst => Some (tyArr tyExpr (tyArr d tySubst))
+	| of_var _ => Some tyVar
+	| of_null => Some tyVal
+    | of_stack_get => Some (tyArr tyVar tyExpr)
+    | of_stack_set => Some (tyArr tyVar (tyArr tyVal (tyArr tyStack tyStack)))
+    | of_single_subst => Some (tyArr tyExpr (tyArr tyVar tySubst))
     | of_subst => Some (tyArr tySubstList tySubst)
     | of_trunc_subst => Some (tyArr tySubstList tySubst)
 	end.
 
-  Global Instance RelDec_open_func : RelDec (@eq open_func) :=
+  Global Instance RelDec_open_func : RelDec (@eq (open_func typ)) :=
   { rel_dec := fun a b =>
 	         match a, b with
 	  	       | of_const t, of_const t'
 	  	       | of_apply_subst t, of_apply_subst t' => t ?[eq] t'
 	  	       | of_ap t u, of_ap t' u' => (t ?[eq] t' && u ?[eq] u')%bool
+	  	       | of_var v, of_var v' => v ?[ eq ] v'
+	  	       | of_null, of_null
 	  	       | of_stack_get, of_stack_get
 	  	       | of_stack_set, of_stack_set
 	  	       | of_single_subst, of_single_subst
@@ -159,7 +205,7 @@ Section OpenFuncInst.
   Proof.
     constructor.
     destruct x; destruct y; simpl; try rewrite andb_true_iff;
-    repeat rewrite rel_dec_correct; intuition congruence.
+    repeat rewrite rel_dec_correct; try intuition congruence.
   Qed.
   
 	Local Instance Applicative_Fun A : Applicative (Fun A) :=
@@ -232,7 +278,7 @@ Section OpenFuncInst.
 	 Defined.
 *)
 
-	Global Program Instance RSym_OpenFunc : SymI.RSym open_func := {
+	Global Program Instance RSym_OpenFunc : SymI.RSym (open_func typ) := {
 	  typeof_sym := typeof_open_func;
 	  symD := _;
 	  sym_eqb := (fun a b => Some (rel_dec a b))
@@ -245,23 +291,25 @@ Section OpenFuncInst.
 		+ apply typ3_cast_bin.
 		  unfold tyArr. repeat rewrite typ2_cast. unfold Fun.
 		  apply (@ap (Fun stack) (Applicative_Fun _) (typD t) (typD t0)).
+		+ apply t.
+		+ apply HV.
 		+ apply typ2_cast_bin.
 	      unfold tyArr. rewrite typ2_cast.
-	      apply (fun (x : typD d) (s : stack) => s x).
+	      apply (fun (x : typD tyVar) (s : stack) => s x).
 		+ unfold tyArr; repeat rewrite typ2_cast; unfold Fun.
-	 	  pose (@stack_add (typD d) _ (@VN typ _ r null)). apply s.
+	 	  pose (@stack_add (typD tyVar) (typD tyVal) _). apply s.
 		+ unfold tyArr; repeat rewrite typ2_cast; unfold Fun.
 	  	  rewrite stSubst.
-		  apply (@apply_subst (typD d) (@VN typ _ r null) (typD t)).
+		  apply (@apply_subst (typD tyVar) (typD tyVal) (typD t)).
 		+ unfold tyArr; repeat rewrite typ2_cast; unfold Fun.
 		  rewrite stSubst.
-		  apply (@subst1 (typD d) _ (@VN typ _ r null)).
+		  apply (@subst1 (typD tyVar) (typD tyVal) _).
 		+ unfold tyArr; rewrite typ2_cast; unfold Fun.
 	      rewrite btList, btPair, stSubst; repeat rewrite typ2_cast.
-	      apply (@substl_aux (typD d) _ (@VN typ _ r null)).
+	      apply (@substl_aux (typD tyVar) (typD tyVal) _).
 		+ unfold tyArr; rewrite typ2_cast; unfold Fun.
 		  rewrite btList, btPair, stSubst. repeat rewrite typ2_cast.
-		  apply (@substl_trunc_aux (typD d) _ (@VN typ _ r null)).
+		  apply (@substl_trunc_aux (typD tyVar) (typD tyVal) _ _).
 	Defined.
 
   Global Instance RSymOk_lopen_func : SymI.RSymOk RSym_OpenFunc.
@@ -274,9 +322,14 @@ Section OpenFuncInst.
 End OpenFuncInst.
 
 Section MakeOpen.
-	Context {typ func : Type} {H : OpenFunc typ func} {H1 : ListFunc typ func}
+	Context {typ func : Type} {HR : RType typ} {HS : SubstType typ}.
+	Context {H : OpenFunc typ func} {H1 : ListFunc typ func}
 	        {HBT : BaseType typ}.
 
+    Context  {Typ2_tyArr : Typ2 _ Fun}.
+    Let tyArr : typ -> typ -> typ := @typ2 _ _ _ _.
+
+	Definition mkVar (v : typD tyVar) : expr typ func := Inj (fVar v). 
 	Definition mkConst (t : typ) (e : expr typ func) := App (fConst t) e.
 	Definition mkAp (t u : typ) (f e : expr typ func) := App (App (fAp t u) f) e.
 	Definition mkStackGet (x s : expr typ func) := App (App fStackGet x) s.
@@ -287,5 +340,11 @@ Section MakeOpen.
 	Definition mkSubst (s : expr typ func) := App fSubst s.
 	Definition mkTruncSubst (s : expr typ func) := App fTruncSubst s.
 	Definition mkApplyTruncSubst t P s := mkApplySubst t P (mkTruncSubst s).
+			
+	Fixpoint mkAps f es t :=
+		match es with 
+			| nil => mkConst t f
+			| (e, t')::es => mkAp t' t (mkAps f es (tyArr t' t)) e
+		end.
 
 End MakeOpen.
