MirrorCharge!/src/MirrorCharge/ModularFunc/SubstType.v
@@ -13,17 +13,17 @@ Set Strict Implicit.
 Set Maximal Implicit Insertion.
 
 Class SubstType (typ : Type) := {
+  tyVar : typ;
+  tyVal : typ;
   tySubst : typ
 }.
 
 Section SubstTypeD.
 	Context {typ : Type} {HT : SubstType typ} {HR : RType typ}.
-	Context {d r : typ} {null : typD r}.
-	
-    Local Instance VN : ValNull := @Build_ValNull (typD r) null.
+	Context {VN : ValNull (typD tyVal)}.
 
 	Class SubstTypeD := {
-	  stSubst : typD tySubst = @subst (typD d) VN
+	  stSubst : typD tySubst = @subst (typD tyVar) (typD tyVal)
 	}.
 	
 End SubstTypeD.
