MirrorCharge!/src/MirrorCharge/RTac/Subst.v
@@ -1,0 +1,148 @@
+Require Import String.
+Require Import ExtLib.Core.RelDec.
+Require Import MirrorCore.Lambda.Expr.
+Require Import MirrorCore.Lambda.AppN.
+Require Import MirrorCore.TypesI.
+Require Import MirrorCore.RTac.RTac.
+Require Import MirrorCore.Lambda.RedAll.
+
+Require Import MirrorCharge.ModularFunc.OpenFunc.
+Require Import MirrorCharge.ModularFunc.ILogicFunc.
+Require Import MirrorCharge.ModularFunc.BILogicFunc.
+Require Import MirrorCharge.ModularFunc.LaterFunc.
+Require Import MirrorCharge.ModularFunc.ListFunc.
+Require Import MirrorCharge.ModularFunc.SubstType.
+
+Set Implicit Arguments.
+Set Strict Implicit.
+
+Section ApplySubst.
+	Context {typ func : Type} {RType_typ : RType typ} {ST : SubstType typ}
+	        {HOF : OpenFunc typ func} {HLF : ListFunc typ func}.
+	Context {RelDec_typ : RelDec (@eq typ)}.
+	Context {RelDec_var : RelDec (@eq (typD tyVar))}.
+
+    Variable Typ2_tyArr : Typ2 _ Fun.
+    Let tyArr : typ -> typ -> typ := @typ2 _ _ _ _.
+
+	Definition applySingleSubst (p : expr typ func) (x y : typD tyVar) e :=
+		if x ?[ eq ] y then e else p.
+		    	
+    Fixpoint applyParSubst (p : expr typ func) (x : typD tyVar) vs es :=
+    	match es with
+    		| App (App f e) es =>
+    			match vs, listS f with
+    				| v :: vs, Some (pCons t) =>
+    					if t ?[ eq ] tyArr tyVar tyVal then
+    						if x ?[ eq ] v then
+    							e
+    						else
+    							applyParSubst p x vs es
+    					else
+    						p
+    				| _, _ => p
+    			end
+    		| _ => p
+    	end.
+    						
+    Fixpoint applyTruncSubst (p : expr typ func) (x : typD tyVar) vs es :=
+    	match es with
+    		| App (App f e) es =>
+    			match vs, listS f with
+    				| v :: vs, Some (pCons t) =>
+    					if t ?[ eq ] tyArr tyVar tyVal then
+    						if x ?[ eq ] v then
+    							e
+    						else
+    							applyParSubst p x vs es
+    					else
+    						fNull
+    				| _, _ => fNull
+    			end
+    		| _ => fNull
+    	end.				
+
+	Definition applySubst (t : typ) (f e : expr typ func) (x : typD tyVar) :=
+		match f with
+		  | App (App g e') y =>
+		  	match open_funcS g, open_funcS y with
+		  	  | Some (of_singleSubst), Some (of_var v) => applySingleSubst e x v e'
+		  	  | _, _ => mkApplySubst t e f
+		  	end
+		  | _ => mkApplySubst t e f
+(*		  | mkApplySubst [t, p, mkSubstList [mkVarList [vs], es]] => applyParSubst p x vs es
+		  | mkApplyTruncSubst [t, p, mkSubstList [mkVarList [vs], es]] => applyTruncSubst x vs es*)
+		end.
+
+End ApplySubst.
+
+Section PushSubst.
+  Context {typ func : Type} {ST : SubstType typ} {RType_typ : RType typ}.
+  Context {OF : OpenFunc typ func} {ILF : ILogicFunc typ func} {BILF : BILogicFunc typ func}.
+  Context {RelDec_var : RelDec (@eq (typD tyVar))}.
+  
+  Variable Typ2_tyArr : Typ2 _ Fun.
+  Let tyArr : typ -> typ -> typ := @typ2 _ _ _ _.
+
+  Variable f : expr typ func.
+
+  Fixpoint pushSubst (e : expr typ func) (t : typ) : expr typ func :=
+    match e with
+    	| App (App g p) q =>
+    		match ilogicS g with
+    			| Some (ilf_and l) => mkAnd l (pushSubst p l) (pushSubst q l)
+    			| Some (ilf_or l) => mkOr l (pushSubst p l) (pushSubst q l)
+    			| Some (ilf_impl l) => mkImpl l (pushSubst p l) (pushSubst q l)
+    			| _ => match open_funcS g with
+		    			 | Some (of_ap t1 t2) => mkAp t1 t2 (pushSubst p (tyArr t1 t2))
+		    			             									 (pushSubst q t2)
+		    			 | _ => match bilogicS g with
+		    			          | Some (bilf_star l) => mkStar l (pushSubst p l) (pushSubst q l)
+		    			          | Some (bilf_wand l) => mkWand l (pushSubst p l) (pushSubst q l)
+		    			 	      | _ => mkApplySubst t e f
+		    			 	    end
+		    		   end
+    		end
+    	| App g x =>
+    		match open_funcS g, open_funcS x with
+    			| Some of_stack_get, Some (of_var y) => applySubst t f e y
+    			| Some (of_const _), _ => e
+    			| _, _ => mkApplySubst t e f
+    		end
+    	| _ => match ilogicS e with
+    		     | Some (ilf_true l) => mkTrue l
+    		     | Some (ilf_false l) => mkFalse l
+    		     | _ => match bilogicS e with
+    		     		  | Some (bilf_emp l) => mkEmp l
+    		     		  | _ => mkApplySubst t e f
+    		     		end
+    		   end
+    end.
+    
+End PushSubst.
+
+Section SubstTac.
+  Context {typ func subst : Type} {ST : SubstType typ} {RType_typ : RType typ}.
+  Context {OF : OpenFunc typ func} {ILF : ILogicFunc typ func} {BILF : BILogicFunc typ func}.
+  Context {RelDec_var : RelDec (@eq (typD tyVar))}.
+  
+  Variable Typ2_tyArr : Typ2 _ Fun.
+  Let tyArr : typ -> typ -> typ := @typ2 _ _ _ _.
+
+	Definition substTac (e : expr typ func) (args : list (expr typ func))
+	: expr typ func :=
+	  match open_funcS e with
+	    | Some (of_apply_subst t) =>
+	      match args with
+	        | e :: f :: nil =>
+	          pushSubst Typ2_tyArr f e t
+	        | _ => apps e args
+	      end
+	    | _ => apps e args
+	  end.
+
+	Definition SUBST := SIMPLIFY (typ := typ) (subst := subst) (fun _ _ => beta_all substTac nil nil).
+
+End SubstTac.
+
+Implicit Arguments SUBST [[ST] [RType_typ] [OF] [ILF] [BILF] [RelDec_var] [Typ2_tyArr]].
